---
title: A Simple Proof to Stirling's Formula
date: 2025-07-01
id: blog0404
tag: math
toc: true
intro: We record a study on the asymptotic behaviour of n!
---

#### The Stirling's Formula

> **Theorem.** We have
>
> $$
> n!\sim \sqrt{2\pi n} \left(\frac{n}{e}\right)^n\quad  \text{as $n\to \infty$}
> $$

#### Preliminary Results as Simple Exercises in Mathematical Analysis

<box>

**Fact 1.** Show that for each $n\in \mathbb N$,

$$
\left( \frac{n+1}{e}\right)^n < n!
$$

</box>

<box>

**Fact 2.** Show that the function

$$
f(x) = \left(1+\frac{1}{x}\right)^{x+\alpha}
$$

is decreasing on $(0,\infty)$ when $\alpha \ge \frac{1}{2}$.

</box>

<box>

**Fact 3.** If $f:(a,b)\to \mathbb R$ is convex, then show that for every $x_1,x_2\in (a,b)$ with $x_1<x_2$, one has

$$
f\left(\frac{x_1+x_2}{2}\right)\leq \frac{1}{x_2-x_1}\int_{x_1}^{x_2}f(t)\,dt\leq \frac{f(x_1)+f(x_2)}{2}.
$$

</box>

<box>

**Fact 4 (Walli's Formula).** Define $I_n=\int_0^{\pi/2}\sin^n x\,dx$ for integer $n\ge0$. Prove that for every $n\ge1, $

$$
I_{2n}=\frac{(2n-1)!!}{(2n)!!}\cdot \frac{\pi}{2}\quad\text{and}\quad I_{2n+1}=\frac{(2n)!!}{(2n+1)!!}.
$$

Hence by considering $I_{2n}/I_{2n+1}$, show that

$$
\lim_{n\to\infty} \frac{1}{2n+1}\left(\frac{(2n)!!}{(2n-1)!!}\right)^2=\frac{\pi}{2}.
$$

</box>

#### Proof of the Statement

##### Motivation

By **Fact 1** we have

$$
\left(1+\frac{1}{n}\right)^n<\frac{e^nn!}{n^n}.
$$

We note that LHS increases to $e$, thus if $\displaystyle b_n:=\frac{e^nn!}{n^n}$ also converges, we should get at least a nonzero limit. To study this, consider the quotient

$$
\frac{b_{n+1}}{b_n}=e\left(\frac{n}{n+1}\right)^n\iff \frac{b_{n}}{b_{n+1}}=\frac{1}{e}\left(1+\frac{1}{n}\right)^n<1.
$$

Therefore $\{b_n\}$ is increasing, however this limit is possibly unbounded.

Next by **Fact 2** we can obtain a decreasing sequence by multiplying $\frac{b_n}{b_{n+1}}=\frac{1}{e}\left(1+\frac{1}{n}\right)^n$ a factor $(1+\frac{1}{n})^{1/2}$:

$$
\frac{b_n}{b_{n+1}} \times \left(1+\frac{1}{n}\right)^{1/2}  =\frac{1}{e}\left(1+\frac{1}{n}\right)^{n+1/2}>1.
\tag*{$(*)$}
$$

Observe that LHS of $(*)$ is the sams as $\displaystyle \frac{b_n/\sqrt{n}}{b_{n+1}/\sqrt{n+1}}$, so instead we try to study the limit of

$$
\boxed{a_n:= \frac{b_n}{\sqrt{n}} = \frac{e^n n!}{n^{n+1/2}}}
$$

##### Proof to Stirling's Formula

Let $\{a_n\}$ be defined as above, now observe that

$$
\begin{align*}
1&<\frac{a_n}{a_{n+1}}=e^{-1}\left(1+\frac{1}{n}\right)^{n+1/2}=\exp\bigg(-1+\Big(n+\frac{1}{2}\Big) \int_{n}^{n+1}\frac{1}{x}\,dx\bigg),
\end{align*}
$$

by **Fact 3** we have $\displaystyle  \int_{n}^{n+1}\frac{1}{x}\,dx\leq\frac{1}{2}\left(\frac{1}{n}+\frac{1}{n+1}\right)$, therefore a simple computation yields

$$
1<\frac{a_n}{a_{n+1}}<e^{\frac{1}{4}\left(\frac{1}{n}-\frac{1}{n+1}\right)}.\tag{$**$}
$$

Thus the first inequality in $(**)$ tells us $\{a_n\}$ converges to a nonnegative limit $\boxed{\alpha:=\lim_{n\to\infty} a_n}$; The second inequality in $(**)$ tell us $\{a_ne^{-\frac{1}{4n}}\}$ increases to $\alpha$, so $\alpha >0$. By using the following form of Walli's formula (modified from **Fact 4**)

$$
\frac{(n!)^2 2^{2n}}{(2n)!}\sim \sqrt{\pi n}
$$

and using $n!=a_nn^{n+1/2}e^{-n}$ we get

$$
\sqrt{\pi}\leftarrow \frac{(n!)^22^{2n}}{\sqrt{n}(2n)!}=\frac{1}{\sqrt{2}} \frac{a_n^2}{a_{2n}}\to \frac{\alpha}{\sqrt{2}}.
$$

Therefore we conclude that

$$
\lim_{n\to\infty} \frac{n!}{n^{n+1/2} e^{-n}}=\lim_{n\to\infty}a_n=\alpha =\sqrt{2\pi}
$$

For the ease of memorization this result is usually written as

<qed>

$$
\boxed{\displaystyle n!\sim \sqrt{2\pi n} \left(\frac{n}{e}\right)^n}.
$$

</qed>
